SierraLean/FuncData/Struct.lean
@@ -1,0 +1,29 @@
+import SierraLean.FuncDataUtil
+
+open Qq Lean Sierra
+
+namespace Sierra.FuncData
+
+private def struct_construct_condition {l} (fields : List (Fin l × SierraType))
+   (fields' : List SierraType) (acc : Expr → Expr := id) :
+    OfInputs Q(Prop) (List.map SierraType.toQuote (fields.map (·.2) ++ [SierraType.Struct fields'])) :=
+match fields with
+| [] => fun (ρ : Expr) => acc ρ
+| ((idx, field) :: fields) => fun a =>
+  let acc' : Expr → Expr := fun ρ =>
+    Expr.mkAnds [acc ρ, Expr.mkEq (SierraType.toQuote field) (mkApp ρ q(0)) a]
+  struct_construct_condition fields fields' acc'
+
+def struct_construct (fields : List SierraType) : FuncData where
+  inputTypes := fields
+  branches := [{ outputTypes := [.Struct fields]
+                 condition := List.map_of_enumFin fields ▸
+                  struct_construct_condition fields.enumFin (Prod.snd <$> fields.enumFin) }]
+
+def structLibFuncs (typeRefs : HashMap Identifier SierraType) : Identifier → Option FuncData
+| .name "struct_construct" [.identifier ident] =>
+  match typeRefs.find? ident with
+  | .some (.Struct fields) => struct_construct fields
+  | _ => .none
+| _ => .none
+
